text/Validatable.dfy
@@ -1,0 +1,34 @@
+module Validation {
+  trait {:termination false} Validatable {
+    ghost var Repr: set<object>
+    // This would include `AllSingletons !in Repr`
+    predicate Valid() reads this, Repr ensures Valid() ==> this in Repr
+  }
+
+  // This would be a singleton to track all valid-by-default objects
+  class AllSingletons {
+    ghost var singletons: set<Validatable>
+    ghost var singletonReprs: set<object>
+
+    predicate AllValid() reads this, singletons, singletonReprs {
+      forall s :: s in singletons ==> this !in s.Repr && s.Repr <= singletonReprs && s.Valid()
+    }
+
+    constructor() ensures AllValid() {
+      singletons := {};
+    }
+
+    method AddSingleton(v: Validatable) 
+      requires AllValid()
+      requires v.Valid()
+      requires this !in v.Repr
+      modifies this
+      ensures v in singletons
+      ensures v.Repr <= singletonReprs
+      ensures AllValid()
+    {
+      singletons := singletons + {v};
+      singletonReprs := singletonReprs + v.Repr;
+    }
+  }
+}
